theories/hoare.v
@@ -396,8 +396,7 @@ Local Notation "c ||> p" := (to_hoare (M:=M) c p)
 Lemma to_hoare_distinguished_trigger_preI (ω : Ω) :
   pre (c ||> ptrigger op) ω.
 Proof.
-by rewrite to_hoare_triggerE /hoare_of_contract /gen_caller_obligation
-  (@injK_None Fx G F).
+by rewrite to_hoare_triggerE /hoare_of_contract /gen_caller_obligation injK_None.
 Qed.
 
 Lemma to_hoare_distinguished_trigger_postE (ω : Ω) (x : A) (ω' : Ω) :
@@ -405,11 +404,61 @@ Lemma to_hoare_distinguished_trigger_postE (ω : Ω) (x : A) (ω' : Ω) :
   ω' = ω.
 Proof.
 by rewrite to_hoare_triggerE /=
-  /gen_witness_update /gen_callee_obligation
-  (@injK_None Fx G F);
+  /gen_witness_update /gen_callee_obligation injK_None;
    split=> [[-> _] | ->].
 Qed.
 End ToHoareDistinguishSection.
+
+(** ** Shared Contract Trigger Views *)
+
+Section ToHoareSharedContractSection.
+Context {F G H : effect} `{StrictProvide2 H F G}
+    {M : freerMonad H} (Ω : Type) (ci : contract F Ω)
+    (cj : contract G Ω).
+
+Lemma to_hoare_shared_contract_left_trigger_preI
+    {A : Type} (op : F A) (ω : Ω) :
+  caller_obligation ci ω op ->
+  pre (to_hoare (M:=M) (ci -^- cj) (ptrigger op)) ω.
+Proof.
+by rewrite to_hoare_triggerE /hoare_of_contract /sharedcontractprod
+  /gen_caller_obligation /= injK_None injK_Some.
+Qed.
+
+Lemma to_hoare_shared_contract_right_trigger_preI
+    {A : Type} (op : G A) (ω : Ω) :
+  caller_obligation cj ω op ->
+  pre (to_hoare (M:=M) (ci -^- cj) (ptrigger op)) ω.
+Proof.
+by rewrite to_hoare_triggerE /hoare_of_contract /sharedcontractprod
+  /gen_caller_obligation /= injK_None injK_Some.
+Qed.
+
+Lemma to_hoare_shared_contract_left_trigger_postE
+    {A : Type} (op : F A)
+    (ω : Ω) (x : A) (ω' : Ω) :
+  post (to_hoare (M:=M) (ci -^- cj) (ptrigger op)) ω x ω' <->
+  ω' = witness_update ci ω op x /\
+  callee_obligation ci ω op x.
+Proof.
+by rewrite to_hoare_triggerE /hoare_of_contract /gen_witness_update
+  /sharedcontractprod /gen_callee_obligation /= injK_Some injK_None;
+  tauto.
+Qed.
+
+Lemma to_hoare_shared_contract_right_trigger_postE
+    {A : Type} (op : G A)
+    (ω : Ω) (x : A) (ω' : Ω) :
+  post (to_hoare (M:=M) (ci -^- cj) (ptrigger op)) ω x ω' <->
+  ω' = witness_update cj ω op x /\
+  callee_obligation cj ω op x.
+Proof.
+by rewrite to_hoare_triggerE /hoare_of_contract /gen_witness_update
+  /sharedcontractprod /gen_callee_obligation /= injK_None injK_Some;
+  tauto.
+Qed.
+
+End ToHoareSharedContractSection.
 
 Global Opaque gen_caller_obligation gen_witness_update gen_callee_obligation.
 Global Opaque hoare_of_contract.
